---
title: Advanced Course in Algorithms - Problem Set 1
author: Jaan Tollander de Balsch
date: \today
header-includes: \usepackage{unicode-math}
---
## Problem 1
### a)
Multiply \(a=x+x^2∈ℤ_2[x]\) and \(b=1+x+x^3∈ℤ_2[x]\).

---

\[
a⋅b=x+x^3+x^4+x^5 ∈ℤ_2[x]
\]

### b)
Divide \(a=1+x^2+x^3+x^4+x^6 ∈ℤ_2[x]\) and \(b=1+x^3+x^4 ∈ℤ_2[x]\). Present a quotient \(q∈ℤ_2[x]\) and a remainder \(r∈ℤ_2[x]\) such that  \(a=q⋅b+r\) and \(\deg r<\deg b.\)

---

First division gives us
\[
a=q_1 b+r_1,
\]
where the quotient \(q_1=x^2\) and the remainder \(r_1=1+x^3+x^4+x^5\). Since \(\deg r_1>\deg b\) we'll divide again. Second division given us
\[
r_1=q_2 b+r_2,
\]
where the quotient \(q_2=x\) and the remainder \(r_2=1+x+x^3\). The division terminates because \(\deg r_2<\deg b\). Lets collect the terms
\[
\begin{aligned}
a &= q_1 b+r_1 \\
&= q_1 b + (q_2 b + r_2) \\
&= (q_1+q_2) b + r_2 \\
&= q b + r.
\end{aligned}
\]
We see that the quotient and the remainder takes the form
\[
\begin{aligned}
q&=q_1+q_2=x+x^2 \\
r&=r_2=1+x+x^3.
\end{aligned}
\]


## Problem 2
### a)
Find the greatest common divisor of \(f=1234567\) and \(g=123\) in \(ℤ\). Using the output of the algorithm, find \(g^{-1}∈ℤ_f.\)

---

Using the Traditional Euclidian algorithm on \(f\) and \(g\) gives us
\[
\begin{aligned}
1234567 &= 10037⋅123+16 \\
123 &= 7⋅16+11 \\
16 &= 1⋅11+5 \\
11 &= 2⋅5+1.
\end{aligned}
\]

Written in another form
\[
\begin{aligned}
1 &= 11 - 2⋅5 \\
5 &= 16 - 1⋅11 \\
11 &= 123 - 7⋅16 \\
16 &= 1234567 - 10037⋅123
\end{aligned}
\]

Now using back substitution on the equation we can obtain coefficients for the Diophantine equation
\[
a⋅f+b⋅g = 1.
\]
where \(a = -23\) and \(b = 230854\).

Written in another form
\[
b⋅g = -a⋅f+1
\]
we see that the coefficient \(b\) is answer for \(g^{-1}∈ℤ_f\) because
\[
\begin{aligned}
g⋅g^{-1}\mod f&=1 \\
g⋅g^{-1}&=k⋅f+1, k∈ℤ_f
\end{aligned}
\]
where \(k=-a=23\) and \(g^{-1}=b=230854.\)


### b)
Find a greatest common divisor of \(f=1+x+x^3+x^4\) and \(g=1+x^4\) in \(ℤ_2[x]\).

---

Using Traditional Euclidian algorithm on \(f\) and \(g\) gives us
\[
\begin{aligned}
1+x+x^3+x^4 &= 1⋅(1+x^4)+(x+x^3) \\
1+x^4 &= x⋅(x+x^3)+(1+x^2) \\
x+x^3 &= x⋅(1+x^2)+0.
\end{aligned}
\]
From the output we can see that
\[
\gcd(f,g)=1+x^2∈ℤ_2[x].
\]


## Problem 3
Let \(ξ_0,ξ_1,…,ξ_d∈F\) be distinct elements in a field \(F\). Show that Vandermonde matrix
\[
Ξ =
\left[\begin{matrix}
ξ_0^0 & ξ_0^1 & … & ξ_0^d \\
ξ_1^0 & ξ_1^1 & … & ξ_1^d \\
⋮ & ⋮ &  & ⋮ \\
ξ_d^0 & ξ_d^1 & … & ξ_d^d \\
\end{matrix}\right]
∈ F^{(d+1)×(d+1)}
\]
is invertible.

---

The Lagrange polynomial \(L(x)∈F[x]\) for \(i=0,1,…,d\) is defined by
\[
L_i(x) = ∏_{j=0,j≠i}^d \frac{x-ξ_j}{ξ_i-ξ_j} = ∑_{k=0}^d λ_{ik} x^k.
\]

Then evaluating it at the point \(x=ξ_m\) where \(m∈\{0,1,…,d\}\) gives us
\[
\begin{aligned}
L_i(ξ_m) &= ∏_{j=0,j≠i}^d \frac{ξ_m-ξ_j}{ξ_i-ξ_j}
\\
& =
\begin{cases}
0, & m≠i \\
1, & m=i
\end{cases}
\\
&= δ_{m,i}
\end{aligned}
\]
and
\[
\begin{aligned}
L_i(ξ_m) &= ∑_{k=0}^d λ_{k,i} ξ_m^k \\
&= ∑_{k=0}^d ξ_m^k λ_{k,i} \\
&=
\left[\begin{matrix}
ξ_m^0 & ξ_m^1 & … & ξ_m^d
\end{matrix}\right]
·
\left[\begin{matrix}
λ_{0,i} \\ λ_{1,i} \\ ⋮ \\ λ_{d,i}
\end{matrix}\right].
\end{aligned}
\]

Written in matrix form over \(i,m∈\{0,1,…,d\}\) gives us
\[
\begin{aligned}
\left[\begin{matrix}
ξ_0^0 & ξ_0^1 & … & ξ_0^d \\
ξ_1^0 & ξ_1^1 & … & ξ_1^d \\
⋮ & ⋮ &  & ⋮ \\
ξ_d^0 & ξ_d^1 & … & ξ_d^d \\
\end{matrix}\right]
⋅
\left[\begin{matrix}
λ_{0,0} & λ_{0,1} & … & λ_{0,d} \\
λ_{1,0} & λ_{1,1} & … & λ_{1,d} \\
⋮ & ⋮ &  & ⋮ \\
λ_{d,0} & λ_{d,1} & … & λ_{d,d} \\
\end{matrix}\right]
&=
\left[\begin{matrix}
δ_{0,0} & δ_{0,1} & … & δ_{0,d} \\
δ_{1,0} & δ_{1,1} & … & δ_{1,d} \\
⋮ & ⋮ &  & ⋮ \\
δ_{d,0} & δ_{d,1} & … & δ_{d,d} \\
\end{matrix}\right]
\\
Ξ⋅𝚲&= 𝐈
\\
𝚲&=Ξ^{-1}.
\end{aligned}
\]
Because the Kronecker delta generates the indentity matrix \(𝐈\), the matrix \(𝚲\) generated by the coefficients \(λ_{i,j}\) is the inverse of \(Ξ\).


## Problem 4
The initial values in the traditional Euclidian algorithm are
\[
\begin{aligned}
r_0=f, s_0=1, t_0=0, \\
r_1=g, s_1=0, t_1=1. \\
\end{aligned}
\]

The subsequent values when \(i≥1\) are given by recursive relationship as
\[
\begin{aligned}
q_i = quo(r_{i-1},r_i), \\
r_{i+1} = r_{i-1} - q_i r_i, \\
s_{i+1} = s_{i-1} - q_i s_i, \\
t_{i+1} = t_{i-1} - q_i t_i.
\end{aligned}
\]

The matrices \(R\) and \(Q\) are defined
\[
\begin{aligned}
R_0 =
\left[\begin{matrix}
s_0 & t_0 \\
s_1 & t_1 \\
\end{matrix}\right]
\end{aligned},
\begin{aligned}
Q_i =
\left[\begin{matrix}
0 & 1 \\
1 & -q_i \\
\end{matrix}\right]
\end{aligned}
, i=1,2,…,l.
\]
and
\[
R_i = Q_i Q_{i-1} ⋯ Q_1 R_0, i=0,1,…,l.
\]

Note that \(Q\) is also invertible
\[
Q_i^{-1}=
\left[\begin{matrix}
q_i & 1 \\
1 & 0
\end{matrix}\right].
\]

Another useful relation is
\[
\begin{aligned}
R_{i+1} &= Q_{i+1} Q_i Q_{i-1} ⋯ Q_1 R_0, i=0,1,…,l \\
&=Q_{i+1} R_i.
\end{aligned}
\]

<!-- \[
\begin{aligned}
r_{i+1} &= r_{i-1} - q_i r_i \\
r_{i+1} + q_i r_i &= r_{i-1} \\
\end{aligned}
\] -->


### a)
Show that invariant holds for all \(i=0,1,…,l\):
\[
R_i
\left[\begin{matrix}
f \\ g
\end{matrix}\right]
=
\left[\begin{matrix}
r_i \\ r_{i+1}
\end{matrix}\right].
\]

Lets show that the **base case** \(i=0\) is true.
\[
\begin{aligned}
R_0
\left[\begin{matrix}
f \\ g
\end{matrix}\right]
&=
\left[\begin{matrix}
r_0 \\ r_{1}
\end{matrix}\right]
\\
\left[\begin{matrix}
1 & 0 \\
0 & 1 \\
\end{matrix}\right]
\left[\begin{matrix}
f \\ g
\end{matrix}\right]
&=
\left[\begin{matrix}
r_0 \\ r_{1}
\end{matrix}\right]
\\
\left[\begin{matrix}
f \\ g
\end{matrix}\right]
&=
\left[\begin{matrix}
r_0 \\ r_{1}
\end{matrix}\right].
\end{aligned}
\]

We will assume that the **case** \(i=n≥1\) is true and show that then also **case** \(i=n+1\) is true.
\[
\begin{aligned}
R_{n+1}
\left[\begin{matrix}
f \\ g
\end{matrix}\right]
&=
\left[\begin{matrix}
r_{n+1} \\ r_{(n+1)+1}
\end{matrix}\right]
\\
Q_{n+1} R_{n}
\left[\begin{matrix}
f \\ g
\end{matrix}\right]
&=
\left[\begin{matrix}
r_{n+1} \\ r_{(n+1)+1}
\end{matrix}\right]
\\
R_{n}
\left[\begin{matrix}
f \\ g
\end{matrix}\right]
&=
Q_{n+1}^{-1}
\left[\begin{matrix}
r_{n+1} \\ r_{(n+1)+1}
\end{matrix}\right]
\\
&=
\left[\begin{matrix}
q_{n+1} & 1 \\
1 & 0
\end{matrix}\right]
\left[\begin{matrix}
r_{n+1} \\ r_{(n+1)+1}
\end{matrix}\right]
\\
&=
\left[\begin{matrix}
q_{n+1} r_{n+1} + r_{n+2} \\ r_{n+1}
\end{matrix}\right]
\\
&=
\left[\begin{matrix}
r_{n} \\ r_{n+1}
\end{matrix}\right].
\end{aligned}
\]

### b)
Show that invariant holds for all \(i=0,1,…,l\):
\[
R_i =
\left[\begin{matrix}
s_i & t_i \\
s_{i+1} & t_{i+1} \\
\end{matrix}\right]
\]

**Base case** \(i=0\) is true by definition. We'll assume case \(i=n≥1\) to be true and then show that \(i=n+1\) is also true.
\[
\begin{aligned}
R_{n+1}
&=
\left[\begin{matrix}
s_{n+1} & t_{n+1} \\
s_{(n+1)+1} & t_{(n+1)+1} \\
\end{matrix}\right]
\\
R_n
&=
Q_{n+1}^{-1}
\left[\begin{matrix}
s_{n+1} & t_{n+1} \\
s_{(n+1)+1} & t_{(n+1)+1} \\
\end{matrix}\right]
\\
&=
\left[\begin{matrix}
q_{n+1} & 1 \\
1 & 0
\end{matrix}\right]
\left[\begin{matrix}
s_{n+1} & t_{n+1} \\
s_{(n+1)+1} & t_{(n+1)+1} \\
\end{matrix}\right]
\\
&=
\left[\begin{matrix}
q_{n+1} s_{n+1} + s_{n+2} & q_{n+1} t_{n+2} + t_{n+1} \\
s_{n+1} & t_{n+1} \\
\end{matrix}\right]
\\
&=
\left[\begin{matrix}
s_n & t_n \\
s_{n+1} & t_{n+1} \\
\end{matrix}\right].
\end{aligned}
\]

### c)
The output of Euclidian algorithm is as follows.
\[
\begin{aligned}
r_0 &= q_1 r_1 +r_2 \\
r_1 &= q_2 r_2 +r_3 \\
r_2 &= q_3 r_3 +r_4 \\
&⋮ \\
r_{l-2} &= q_{l-1} r_{l-1} +r_{l} \\
r_{l-1} &= q_{l} r_{l} +r_{l+1} \\
\end{aligned}
\]

Then the algorithm terminates when \(r_{l+1}=0\). This means that \(r_{l-1}\) is divisible by \(r_l\) which implies that \(r_{l-2}\) is divisible by \(r_l\) and by this logic all \(r_{l-1},…,r_0\) are divisible by \(r_l\). Divisor \(r_l\) must be the greatest common divisor, otherwise there would exists \(i∈[0, l]\) such that \(r_i=0\).


### d)
By using the statements proven in sections (a) and (b) we have
\[
\begin{aligned}
R_i
\left[\begin{matrix}
f \\ g
\end{matrix}\right]
&=
\left[\begin{matrix}
r_i \\ r_{i+1}
\end{matrix}\right]
\\
\left[\begin{matrix}
s_i & t_i \\
s_{i+1} & t_{i+1} \\
\end{matrix}\right]
\left[\begin{matrix}
f \\ g
\end{matrix}\right]
&=
\left[\begin{matrix}
r_i \\ r_{i+1}
\end{matrix}\right]
\\
s_i f + t_i g &= r_i.
\end{aligned}
\]
